cleanups

src/Init/Data/Iterators/Consumers/Loop.lean
@@ -24,13 +24,24 @@ These operations are implemented using the `IteratorLoop` and `IteratorLoopParti
 
 namespace Std.Iterators
 
-instance (α : Type w) (β : Type w) (n : Type w → Type w') [Monad n]
+/--
+A `ForIn'` instance for iterators. Its generic membership relation is not easy to use,
+so this is not marked as `instance`. This way, more convenient instances can be built on top of it
+or future library improvements will make it more comfortable.
+-/
+def Iter.instForIn' {α : Type w} {β : Type w} {n : Type w → Type w'} [Monad n]
     [Iterator α Id β] [Finite α Id] [IteratorLoop α Id n] :
     ForIn' n (Iter (α := α) β) β ⟨fun it out => it.IsPlausibleIndirectOutput out⟩ where
   forIn' it init f :=
     IteratorLoop.finiteForIn' (fun δ (c : Id δ) => pure c.run) |>.forIn' it.toIterM init
         fun out h acc =>
           f out (Iter.isPlausibleIndirectOutput_iff_isPlausibleIndirectOutput_toIterM.mpr h) acc
+
+instance (α : Type w) (β : Type w) (n : Type w → Type w') [Monad n]
+    [Iterator α Id β] [Finite α Id] [IteratorLoop α Id n] :
+    ForIn n (Iter (α := α) β) β :=
+  haveI : ForIn' n (Iter (α := α) β) β _ := Iter.instForIn'
+  instForInOfForIn'
 
 instance (α : Type w) (β : Type w) (n : Type w → Type w') [Monad n]
     [Iterator α Id β] [IteratorLoopPartial α Id n] :
