src/Init/Data/Iterators/Lemmas/Consumers/Monadic/Loop.lean
@@ -19,19 +19,19 @@ theorem IterM.DefaultConsumers.forIn'_eq_match_step {α β : Type w} {m : Type w
     {wf : IteratorLoop.WellFounded α m plausible_forInStep}
     {it : IterM (α := α) m β} {init : γ}
     {f : (b : β) → it.IsPlausibleIndirectOutput b → (c : γ) → n (Subtype (plausible_forInStep b c))} :
-    IterM.DefaultConsumers.forIn lift γ plausible_forInStep wf it init f = (do
+    IterM.DefaultConsumers.forIn' lift γ plausible_forInStep wf it init f = (do
       match ← lift _ it.step with
       | .yield it' out h =>
         match ← f out (.direct ⟨_, h⟩) init with
         | ⟨.yield c, _⟩ =>
-          IterM.DefaultConsumers.forIn lift _ plausible_forInStep wf it' c
+          IterM.DefaultConsumers.forIn' lift _ plausible_forInStep wf it' c
             fun out h'' acc => f out (.indirect ⟨_, rfl, h⟩ h'') acc
         | ⟨.done c, _⟩ => return c
       | .skip it' h =>
-        IterM.DefaultConsumers.forIn lift _ plausible_forInStep wf it' init
+        IterM.DefaultConsumers.forIn' lift _ plausible_forInStep wf it' init
           fun out h' acc => f out (.indirect ⟨_, rfl, h⟩ h') acc
       | .done _ => return init) := by
-  rw [forIn]
+  rw [forIn']
   apply bind_congr
   intro step
   cases step using PlausibleIterStep.casesOn <;> rfl
@@ -40,7 +40,8 @@ theorem IterM.forIn'_eq {α β : Type w} {m : Type w → Type w'} [Iterator α m
     {n : Type w → Type w''} [Monad n] [IteratorLoop α m n] [hl : LawfulIteratorLoop α m n]
     [MonadLiftT m n] {γ : Type w} {it : IterM (α := α) m β} {init : γ}
     {f : (b : β) → it.IsPlausibleIndirectOutput b → γ → n (ForInStep γ)} :
-    ForIn'.forIn' it init f = IterM.DefaultConsumers.forIn (fun _ => monadLift) γ (fun _ _ _ => True)
+    letI : ForIn' n (IterM (α := α) m β) β _ := IterM.instForIn'
+    ForIn'.forIn' it init f = IterM.DefaultConsumers.forIn' (fun _ => monadLift) γ (fun _ _ _ => True)
         IteratorLoop.wellFounded_of_finite it init ((⟨·, .intro⟩) <$> f · · ·) := by
   cases hl.lawful; rfl
 
@@ -48,7 +49,7 @@ theorem IterM.forIn_eq {α β : Type w} {m : Type w → Type w'} [Iterator α m 
     {n : Type w → Type w''} [Monad n] [IteratorLoop α m n] [hl : LawfulIteratorLoop α m n]
     [MonadLiftT m n] {γ : Type w} {it : IterM (α := α) m β} {init : γ}
     {f : β → γ → n (ForInStep γ)} :
-    ForIn.forIn it init f = IterM.DefaultConsumers.forIn (fun _ => monadLift) γ (fun _ _ _ => True)
+    ForIn.forIn it init f = IterM.DefaultConsumers.forIn' (fun _ => monadLift) γ (fun _ _ _ => True)
         IteratorLoop.wellFounded_of_finite it init (fun out _ acc => (⟨·, .intro⟩) <$> f out acc) := by
   cases hl.lawful; rfl
 
@@ -57,6 +58,7 @@ theorem IterM.forIn'_eq_match_step {α β : Type w} {m : Type w → Type w'} [It
     [IteratorLoop α m n] [LawfulIteratorLoop α m n]
     [MonadLiftT m n] {γ : Type w} {it : IterM (α := α) m β} {init : γ}
     {f : (out : β) → _ → γ → n (ForInStep γ)} :
+    letI : ForIn' n (IterM (α := α) m β) β _ := IterM.instForIn'
     ForIn'.forIn' it init f = (do
       match ← it.step with
       | .yield it' out h =>
